Prove Wellformed.update upto lemmas on ReactorType.Equivalent

src/ReactorModel/Objects/Reactor/ReactorType/Equivalent.lean
@@ -2,39 +2,69 @@ import ReactorModel.Objects.Reactor.ReactorType.Indexable
 
 namespace ReactorType
 
+-- TODO: Perhaps find another definition (that also works well with `LawfulUpdatable`). For example,
+--       `con?_id_eq` doesn't seem to be useful.
 structure Equivalent [Indexable α] (rtr₁ rtr₂ : α) : Prop where
-  con? : ∀ cmp, rtr₁[cmp]&.map (·.id) = rtr₂[cmp]&.map (·.id)
-  rcns : rtr₁[.rcn] = rtr₂[.rcn]
+  con?_id_eq : ∀ cmp, rtr₁[cmp]&.map (·.id) = rtr₂[cmp]&.map (·.id)
+  rcns_eq    : rtr₁[.rcn] = rtr₂[.rcn]
 
 namespace Equivalent
 
-variable [Indexable α]
+variable [Indexable α] {rtr rtr₁ : α}
 
 instance : HasEquiv α where 
   Equiv := Equivalent
 
 @[refl]
-protected theorem refl {rtr : α} : rtr ≈ rtr where
-  con? _ := rfl
-  rcns   := rfl
+protected theorem refl : rtr ≈ rtr where
+  con?_id_eq _ := rfl
+  rcns_eq      := rfl
 
 @[symm]
-protected theorem symm {rtr₁ : α} (e : rtr₁ ≈ rtr₂) : rtr₂ ≈ rtr₁ where
-  con? cmp := e.con? cmp |>.symm
-  rcns     := e.rcns.symm
+protected theorem symm (e : rtr₁ ≈ rtr₂) : rtr₂ ≈ rtr₁ where
+  con?_id_eq cmp := e.con?_id_eq cmp |>.symm
+  rcns_eq        := e.rcns_eq.symm
 
 @[trans]
-protected theorem trans {rtr₁ : α} (e₁ : rtr₁ ≈ rtr₂) (e₂ : rtr₂ ≈ rtr₃) : rtr₁ ≈ rtr₃ where
-  con? cmp := e₁.con? cmp |>.trans (e₂.con? cmp)
-  rcns     := e₁.rcns.trans e₂.rcns
+protected theorem trans (e₁ : rtr₁ ≈ rtr₂) (e₂ : rtr₂ ≈ rtr₃) : rtr₁ ≈ rtr₃ where
+  con?_id_eq cmp := e₁.con?_id_eq cmp |>.trans (e₂.con?_id_eq cmp)
+  rcns_eq        := e₁.rcns_eq.trans e₂.rcns_eq
 
-theorem obj?_some_iff {rtr₁ : α} {cmp i} (e : rtr₁ ≈ rtr₂) :
+theorem mem_obj?_ids_iff {cmp i} (e : rtr₁ ≈ rtr₂) : 
+    (i ∈ rtr₁[cmp].ids) ↔ (i ∈ rtr₂[cmp].ids) := by
+  sorry
+
+theorem mem_cmp?_ids_iff {cmp} (e : rtr₁ ≈ rtr₂) : 
+    (i ∈ (cmp? cmp rtr₁).ids) ↔ (i ∈ (cmp? cmp rtr₂).ids) := by
+  sorry
+
+theorem nested (e : rtr₁ ≈ rtr₂) (h₁ : rtr₁[.rtr][i] = some n₁) (h₂ : rtr₂[.rtr][i] = some n₂) : 
+    n₁ ≈ n₂ := 
+  sorry
+
+theorem nest (e : rtr₁ ≈ rtr₂) (h₁ : nest rtr₁ i = some n₁) (h₂ : nest rtr₂ i = some n₂) : 
+    n₁ ≈ n₂ := 
+  sorry
+
+theorem nested_rcns_eq (e : rtr₁ ≈ rtr₂) (h : cmp? .rcn rtr₂ i = some o) : cmp? .rcn rtr₁ i = some o :=
+  sorry
+
+theorem cmp?_some_iff {cmp i} (e : rtr₁ ≈ rtr₂) :
+    (∃ o₁, cmp? cmp rtr₁ i = some o₁) ↔ (∃ o₂, cmp? cmp rtr₂ i = some o₂) := 
+  sorry
+
+theorem obj?_some_iff {cmp i} (e : rtr₁ ≈ rtr₂) :
     (∃ o₁, rtr₁[cmp][i] = some o₁) ↔ (∃ o₂, rtr₂[cmp][i] = some o₂) := 
   sorry
 
-theorem obj?_none_iff {rtr₁ : α} {cmp i} (e : rtr₁ ≈ rtr₂) : 
+theorem obj?_none_iff {cmp i} (e : rtr₁ ≈ rtr₂) : 
     (rtr₁[cmp][i] = none) ↔ (rtr₂[cmp][i] = none) := by 
   sorry
 
 end Equivalent
+
+theorem LawfulUpdate.equiv [Indexable α] {rtr₁ : α} {cmp f} (u : LawfulUpdate cmp i f rtr₁ rtr₂) : 
+    rtr₁ ≈ rtr₂ := 
+  sorry
+
 end ReactorType
