src/ReactorModel/Objects/Reactor/Raw.lean
@@ -7,7 +7,7 @@ namespace Reactor
 
 protected structure Raw where
   core : Reactor.Core
-  uniqueIDs : ReactorType.UniqueIDs core
+  unique_ids : ReactorType.UniqueIDs core
 
 namespace Raw
 
@@ -20,9 +20,9 @@ instance : ReactorType Reactor.Raw where
   nest rtr := 
     (nest rtr.core).attach.map fun ⟨core, h⟩ => {
       core := core
-      uniqueIDs := {
+      unique_ids := {
         allEq := fun l₁ l₂ => 
-          by injection rtr.uniqueIDs.allEq (.nest h.choose_spec l₁) (.nest h.choose_spec l₂)
+          by injection rtr.unique_ids.allEq (.nest h.choose_spec l₁) (.nest h.choose_spec l₂)
       }
     }
 
@@ -31,15 +31,15 @@ instance : ReactorType.LawfulCoe Reactor.Raw Reactor.Core where
   coe := Reactor.Raw.core
 
 instance : ReactorType.Indexable Reactor.Raw where
-  uniqueIDs := ReactorType.UniqueIDs.lift (β := Reactor.Core) $ Reactor.Raw.uniqueIDs ‹_› 
+  unique_ids := ReactorType.UniqueIDs.lift (β := Reactor.Core) $ Reactor.Raw.unique_ids ‹_› 
 
 open ReactorType Updatable in
 noncomputable instance : ReactorType.Updatable Reactor.Raw where
   update rtr cmp i f := {
     core := update rtr.core cmp i f
-    uniqueIDs := UniqueIDs.updated (lawfulUpdate (α := Reactor.Core) rtr cmp i f) rtr.uniqueIDs
+    unique_ids := UniqueIDs.updated (lawful (α := Reactor.Core) rtr cmp i f) rtr.unique_ids
   }
-  lawfulUpdate rtr cmp i f := by exact lawfulUpdate (α := Reactor.Core) rtr cmp i f |>.lift
+  lawful rtr cmp i f := by exact lawful (α := Reactor.Core) rtr cmp i f |>.lift
 
 end Raw
 end Reactor
